cedar-lean/Cedar/Thm/TPE.lean
@@ -52,7 +52,7 @@ theorem partial_evaluate_is_sound
   intro h₁ h₂ h₃
   induction h₁
   case val =>
-    exact partial_evaluate_is_sound_val h₃
+    exact partial_evaluate_is_sound_val
   case var =>
     exact partial_evaluate_is_sound_var h₃
   case ite x₁ x₂ x₃ hwt _ _ hₜ _ hᵢ₁ hᵢ₂ hᵢ₃ =>
